Finish fixing most of the parser
It now mostly works with the new StringLike.

I think I should go back to parameterizing it on the type of characters,
though.  This allows the interface to have a grammar in the context that
mentions only the type of characters, and to put the stringlike bits
inside the interface.

src/Parsers/BooleanRecognizer.v
@@ -1,99 +1,85 @@
 (** * Definition of a boolean-returning CFG parser-recognizer *)
-Require Import Coq.omega.Omega.
-Require Import Coq.Lists.List Coq.Program.Program Coq.Program.Wf Coq.Arith.Wf_nat Coq.Arith.Compare_dec Coq.Classes.RelationClasses Coq.Strings.String.
-Require Import ADTSynthesis.Parsers.ContextFreeGrammar ADTSynthesis.Parsers.ContextFreeGrammarNotations.
+Require Import Coq.Lists.List.
+Require Import Coq.Numbers.Natural.Peano.NPeano Coq.Arith.Compare_dec Coq.Arith.Wf_nat.
+Require Import ADTSynthesis.Parsers.ContextFreeGrammar.
 Require Import ADTSynthesis.Parsers.BaseTypes ADTSynthesis.Parsers.BooleanBaseTypes.
-Require Import ADTSynthesis.Parsers.Grammars.Trivial ADTSynthesis.Parsers.Grammars.ABStar.
-Require Import ADTSynthesis.Parsers.Splitters.RDPList ADTSynthesis.Parsers.Splitters.BruteForce.
+Require Import ADTSynthesis.Parsers.StringLike.Properties.
 Require Import ADTSynthesis.Common ADTSynthesis.Common.Wf.
 
 Set Implicit Arguments.
 Local Open Scope string_like_scope.
 
-(** TODO: Allow stubbing out of individual sub-parse methods *)
 Section recursive_descent_parser.
-  Context {CharType}
-          {String : string_like CharType}
-          {G : grammar CharType}.
-  Context `{data : @boolean_parser_dataT _ String}.
+  Context {string} {HSL : StringLike string} {HSLP : StringLikeProperties string} {G : grammar string}.
+  Context {data : @boolean_parser_dataT string _}.
 
   Section bool.
     Section parts.
       Definition parse_item
-                 (str_matches_nonterminal : string -> bool)
-                 (str : StringWithSplitState String split_stateT)
-                 (it : item CharType)
+                 (str_matches_nonterminal : String.string -> bool)
+                 (str : String)
+                 (it : item string)
       : bool
         := match it with
-             | Terminal ch => [[ ch ]] =s str
+             | Terminal ch => str ~= [ ch ]
              | NonTerminal nt => str_matches_nonterminal nt
            end.
 
       Section production.
         Context {str0}
                 (parse_nonterminal
-                 : forall (str : StringWithSplitState String split_stateT),
+                 : forall (str : String),
                      str ≤s str0
-                     -> string
+                     -> String.string
                      -> bool).
 
         (** To match a [production], we must match all of its items.
             But we may do so on any particular split. *)
         Fixpoint parse_production
-                 (str : StringWithSplitState String split_stateT)
+                 (str : String)
                  (pf : str ≤s str0)
-                 (prod : production CharType)
+                 (prod : production string)
         : bool.
         Proof.
           refine
             match prod with
               | nil =>
                 (** 0-length production, only accept empty *)
-                str =s Empty _
+                Nat.eq_dec (length str) 0
               | it::its
                 => let parse_production' := fun str pf => parse_production str pf its in
                    fold_right
                      orb
                      false
-                     (let mapF f := map f (combine_sig (split_string_for_production_correct it its str)) in
-                      mapF (fun s1s2p =>
-                              (parse_item
-                                 (parse_nonterminal (fst (proj1_sig s1s2p)) _)
-                                 (fst (proj1_sig s1s2p))
-                                 it)
-                                && parse_production' (snd (proj1_sig s1s2p)) _)%bool)
+                     (map (fun n =>
+                             (parse_item
+                                (parse_nonterminal (str := take n str) _)
+                                (take n str)
+                                it)
+                               && parse_production' (drop n str) _)%bool
+                          (split_string_for_production it its str))
             end;
-          revert pf; clear; intros;
-          abstract (
-              destruct str;
-              repeat first [ progress destruct_head sig
-                           | progress destruct_head and
-                           | etransitivity; eassumption
-                           | etransitivity; try eassumption; []
-                           | progress subst
-                           | idtac; match goal with H : (_ =s _) = true |- _ => apply bool_eq_correct in H end
-                           | apply str_le1_append
-                           | apply str_le2_append ]
-            ).
+          revert pf; clear -HSLP; intros;
+          abstract (rewrite ?str_le_take, ?str_le_drop; assumption).
         Defined.
       End production.
 
       Section productions.
         Context {str0}
                 (parse_nonterminal
-                 : forall (str : StringWithSplitState String split_stateT)
+                 : forall (str : String)
                           (pf : str ≤s str0),
-                     string -> bool).
+                     String.string -> bool).
 
         (** To parse as a given list of [production]s, we must parse as one of the [production]s. *)
         Definition parse_productions
-                   (str : StringWithSplitState String split_stateT)
+                   (str : String)
                    (pf : str ≤s str0)
-                   (prods : productions CharType)
+                   (prods : productions string)
         : bool
           := fold_right orb
                         false
-                        (map (parse_production parse_nonterminal str pf)
+                        (map (parse_production parse_nonterminal pf)
                              prods).
       End productions.
 
@@ -103,25 +89,24 @@ Section recursive_descent_parser.
           Context {str0 valid}
                   (parse_nonterminal
                    : forall (p : String * nonterminals_listT),
-                       prod_relation (ltof _ Length) nonterminals_listT_R p (str0, valid)
-                       -> forall str : StringWithSplitState String split_stateT,
-                            str ≤s fst p -> string -> bool).
+                       prod_relation (ltof _ length) nonterminals_listT_R p (str0, valid)
+                       -> forall str : String,
+                            str ≤s fst p -> String.string -> bool).
 
           Definition parse_nonterminal_step
-                     (str : StringWithSplitState String split_stateT)
+                     (str : String)
                      (pf : str ≤s str0)
-                     (nt : string)
+                     (nt : String.string)
           : bool.
           Proof.
             refine
-              (if lt_dec (Length str) (Length str0)
+              (if lt_dec (length str) (length str0)
                then (** [str] got smaller, so we reset the valid nonterminals list *)
                  parse_productions
                    (@parse_nonterminal
                       (str : String, initial_nonterminals_data)
                       (or_introl _))
-                   _
-                   (or_intror eq_refl)
+                   (or_intror (reflexivity _))
                    (Lookup G nt)
                else (** [str] didn't get smaller, so we cache the fact that we've hit this nonterminal already *)
                  if Sumbool.sumbool_of_bool (is_valid_nonterminal valid nt)
@@ -130,7 +115,7 @@ Section recursive_descent_parser.
                      (@parse_nonterminal
                         (str0 : String, remove_nonterminal valid nt)
                         (or_intror (conj eq_refl (remove_nonterminal_dec _ nt _))))
-                     str
+                     (str := str)
                      _
                      (Lookup G nt)
                  else (** oops, we already saw this nonterminal in the past.  ABORT! *)
@@ -143,114 +128,27 @@ Section recursive_descent_parser.
           (** TODO: add comment explaining signature *)
           Definition parse_nonterminal_or_abort
           : forall (p : String * nonterminals_listT)
-                   (str : StringWithSplitState String split_stateT),
+                   (str : String),
               str ≤s fst p
-              -> string
+              -> String.string
               -> bool
             := Fix3
                  _ _ _
                  (well_founded_prod_relation
-                    (well_founded_ltof _ Length)
+                    (well_founded_ltof _ length)
                     ntl_wf)
                  _
                  (fun sl => @parse_nonterminal_step (fst sl) (snd sl)).
 
           Definition parse_nonterminal
-                     (str : StringWithSplitState String split_stateT)
-                     (nt : string)
+                     (str : String)
+                     (nt : String.string)
           : bool
             := @parse_nonterminal_or_abort
                  (str : String, initial_nonterminals_data) str
-                 (or_intror eq_refl) nt.
+                 (or_intror (reflexivity _)) nt.
         End wf.
       End nonterminals.
     End parts.
   End bool.
 End recursive_descent_parser.
-
-(** TODO: move this elsewhere *)
-Section example_parse_string_grammar.
-  Context (G : grammar Ascii.ascii).
-
-  Definition brute_force_parse_nonterminal
-  : @String Ascii.ascii string_stringlike
-    -> string
-    -> bool
-    := let data := @brute_force_data G in parse_nonterminal (G := G).
-
-  Definition brute_force_parse
-  : string -> bool
-    := fun str => brute_force_parse_nonterminal str G.
-End example_parse_string_grammar.
-
-Module example_parse_empty_grammar.
-  Definition parse : string -> bool
-    := brute_force_parse (trivial_grammar _).
-
-  Time Compute parse "".
-  Check eq_refl : true = parse "".
-  Time Compute parse "a".
-  Check eq_refl : false = parse "a".
-  Time Compute parse "aa".
-  Check eq_refl : false = parse "aa".
-End example_parse_empty_grammar.
-
-Section examples.
-  Section ab_star.
-    Local Open Scope string_scope.
-
-    Definition parse : string -> bool
-      := brute_force_parse ab_star_grammar.
-
-    Time Eval lazy in parse "".
-    Check eq_refl : parse "" = true.
-    Time Eval lazy in parse "a".
-    Check eq_refl : parse "a" = false.
-    Time Eval lazy in parse "ab".
-    Check eq_refl : parse "ab" = true.
-    Time Eval lazy in parse "aa".
-    Check eq_refl : parse "aa" = false.
-    Time Eval lazy in parse "ba".
-    Check eq_refl : parse "ba" = false.
-    Time Eval lazy in parse "aba".
-    Check eq_refl : parse "aba" = false.
-    Time Eval lazy in parse "abab".
-    Time Eval lazy in parse "ababab".
-    Check eq_refl : parse "ababab" = true.
-  (* For debugging: *)(*
-    Goal True.
-    pose proof (eq_refl (parse "")) as s.
-    unfold parse in s.
-    unfold brute_force_parse, brute_force_parse_nonterminal in s.
-    cbv beta zeta delta [parse_nonterminal] in s.
-    cbv beta zeta delta [parse_nonterminal_or_abort] in s.
-    rewrite Fix3_eq in s.
-    Ltac do_compute_in c H :=
-      let c' := fresh in
-      set (c' := c) in H;
-        compute in c';
-        subst c'.
-    Tactic Notation "do_compute" open_constr(c) "in" ident(H) :=
-      match type of H with
-        | appcontext[?c0] => unify c c0
-      end;
-      do_compute_in c H.
-    cbv beta zeta delta [parse_nonterminal_step] in s.
-    change (fst (?a, ?b)) with a in s.
-    change (snd (?a, ?b)) with b in s.
-    unfold split_stateT, brute_force_data, default_string_with_no_state, default_String_with_no_state in s.
-    repeat change (string_val {| string_val := ?x |}) with x in s.
-    do_compute_in (Start_symbol ab_star_grammar) s.
-    do_compute_in (@Length Ascii.ascii string_stringlike "ab_star") s.
-    do_compute (lt_dec _ _) in s.
-    cbv beta iota zeta in s.
-    unfold is_valid_nonterminal, initial_nonterminals_data in s.
-    do_compute (is_valid_nonterminal initial_nonterminals_data "") in s.
-    set (n := @Length Ascii.ascii string_stringlike ab_star_grammar) in s.
-    pose ((Length ab_star_grammar)).
-    do_compute_in (Length ab_star_grammar) s.
-    do_compute_in (lt_dec (Length ab_star_grammar) (Length string_stringlike "abab"%string)) s.
-    change (if in_right then ?x else ?y) with y in s.
-    cbv beta zeta delta [rdp_list_is_valid_nonterminal] in s.*)
-  End ab_star.
-End examples.
