src/Parsers/ContextFreeGrammarProperties.v
@@ -1,7 +1,8 @@
 (** * Properties about Context Free Grammars *)
+Require Import Coq.Numbers.Natural.Peano.NPeano.
 Require Import ADTSynthesis.Parsers.StringLike ADTSynthesis.Parsers.ContextFreeGrammar.
 Require Import Coq.Classes.RelationClasses.
-Require Import ADTSynthesis.Common.
+Require Import ADTSynthesis.Common ADTSynthesis.Common.UIP.
 
 Set Implicit Arguments.
 
@@ -10,20 +11,46 @@ Local Open Scope list_scope.
 Section cfg.
   Context {string} `{HSL : StringLike string} `{HSLP : @StringLikeProperties string HSL} (G : grammar string).
 
-  Fixpoint parse_of_respectful (str1 str2 : String) (H : str1 =s str2) (pats : productions string) (p : parse_of G str1 pats) : parse_of G str2 pats
+  Definition parse_of_item_respectful'
+             (parse_of_respectful : forall {str1 str2} (H : str1 =s str2) {pats} (p : parse_of G str1 pats), parse_of G str2 pats)
+             {str1 str2} (H : str1 =s str2) {it} (p : parse_of_item G str1 it)
+  : parse_of_item G str2 it
+    := match p in (parse_of_item _ _ it) return parse_of_item G str2 it with
+         | ParseTerminal ch pf => ParseTerminal G str2 ch (transitivity (eq_sym (is_char_Proper H eq_refl)) pf)
+         | ParseNonTerminal nt p' => ParseNonTerminal _ (parse_of_respectful H p')
+          end.
+
+  Fixpoint parse_of_respectful {str1 str2} (H : str1 =s str2) {pats} (p : parse_of G str1 pats) : parse_of G str2 pats
     := match p in (parse_of _ _ pats) return parse_of G str2 pats with
          | ParseHead pat pats p' => ParseHead pats (parse_of_production_respectful H p')
          | ParseTail pat pats p' => ParseTail pat (parse_of_respectful H p')
        end
-  with parse_of_production_respectful (str1 str2 : String) (H : str1 =s str2) (pat : production string) (p : parse_of_production G str1 pat) : parse_of_production G str2 pat
+  with parse_of_production_respectful {str1 str2} (H : str1 =s str2) {pat} (p : parse_of_production G str1 pat) : parse_of_production G str2 pat
        := match p in (parse_of_production _ _ pat) return parse_of_production G str2 pat with
             | ParseProductionNil pf => ParseProductionNil G str2 (transitivity (eq_sym (length_Proper H)) pf)
-            | ParseProductionCons n pat pats p0 p1 => ParseProductionCons _ n (parse_of_item_respectful (take_Proper eq_refl H) p0) (parse_of_production_respectful (drop_Proper eq_refl H) p1)
+            | ParseProductionCons n pat pats p0 p1 => ParseProductionCons _ n (parse_of_item_respectful' (@parse_of_respectful) (take_Proper eq_refl H) p0) (parse_of_production_respectful (drop_Proper eq_refl H) p1)
+          end.
+
+  Definition parse_of_item_respectful : forall {str1 str2} H {it} p, _
+    := @parse_of_item_respectful' (@parse_of_respectful).
+
+  Fixpoint parse_of_respectful_refl {str pf pats} (p : parse_of G str pats) : parse_of_respectful pf p = p
+    := match p return parse_of_respectful pf p = p with
+         | ParseHead pat pats p' => f_equal (ParseHead _) (parse_of_production_respectful_refl p')
+         | ParseTail pat pats p' => f_equal (@ParseTail _ _ _ _ _ _) (parse_of_respectful_refl p')
+       end
+  with parse_of_production_respectful_refl {str pf pat} (p : parse_of_production G str pat) : parse_of_production_respectful pf p = p
+       := match p return parse_of_production_respectful pf p = p with
+            | ParseProductionNil pf => f_equal (ParseProductionNil _ _) (dec_eq_uip (Nat.eq_dec _) _ _)
+            | ParseProductionCons n pat pats p0 p1
+              => f_equal2 (@ParseProductionCons _ _ _ _ _ _ _)
+                          (parse_of_item_respectful_refl p0)
+                          (parse_of_production_respectful_refl p1)
           end
-  with parse_of_item_respectful (str1 str2 : String) (H : str1 =s str2) (it : item string) (p : parse_of_item G str1 it) : parse_of_item G str2 it
-       := match p in (parse_of_item _ _ it) return parse_of_item G str2 it with
-            | ParseTerminal ch pf => ParseTerminal G str2 ch (transitivity (eq_sym (is_char_Proper H eq_refl)) pf)
-            | ParseNonTerminal nt p' => ParseNonTerminal _ (parse_of_respectful H p')
+  with parse_of_item_respectful_refl {str pf it} (p : parse_of_item G str it) : parse_of_item_respectful pf p = p
+       := match p return parse_of_item_respectful pf p = p with
+            | ParseTerminal ch pf => f_equal (ParseTerminal _ _ _) (dec_eq_uip (Bool.bool_dec _) _ _)
+            | ParseNonTerminal nt p' => f_equal (ParseNonTerminal _) (parse_of_respectful_refl p')
           end.
 
   (*Global Instance parse_of_Proper : Proper (beq ==> eq ==> iff) (parse_of G).
@@ -103,72 +130,74 @@ Section cfg.
     Context {P P' : String -> String.string -> Type}.
 
     Definition expand_forall_parse_of_item'
-               {str}
+               {str str' str''}
                {Forall_parse_of : forall P {str pats} (p : parse_of G str pats), Type}
-               (expand : forall {pats p}, @Forall_parse_of P str pats p -> @Forall_parse_of P' str pats p)
-               (f : forall n, P str n -> P' str n)
-               {it p}
-    : @Forall_parse_of_item' P (@Forall_parse_of P) str it p
-      -> @Forall_parse_of_item' P' (@Forall_parse_of P') str it p.
+               (expand : forall {pats} (H : str =s str') (H' : str =s str'') {p}, @Forall_parse_of P str' pats (parse_of_respectful H p) -> @Forall_parse_of P' str'' pats (parse_of_respectful H' p))
+               (f : forall n, P str' n -> P' str'' n)
+               {it p} (H : str =s str') (H' : str =s str'')
+    : @Forall_parse_of_item' P (@Forall_parse_of P) str' it (parse_of_item_respectful H p)
+      -> @Forall_parse_of_item' P' (@Forall_parse_of P') str'' it (parse_of_item_respectful H' p).
     Proof.
       destruct p; simpl.
       { exact (fun x => x). }
       { intro ab.
-        exact (f _ (fst ab), expand _ _ (snd ab)). }
+        exact (f _ (fst ab), expand _ H H' _ (snd ab)). }
     Defined.
 
     Global Arguments expand_forall_parse_of_item' : simpl never.
 
     Fixpoint expand_forall_parse_of
-             str
-             (f : forall str', str' ≤s str -> forall n, P str' n -> P' str' n)
-             pats (p : parse_of G str pats)
+             str str' str''
+             (f : forall str0' str1', str0' ≤s str -> str0' =s str1' -> forall n, P str0' n -> P' str1' n)
+             pats (H : str =s str') (H' : str =s str'') (p : parse_of G str pats)
              {struct p}
-    : Forall_parse_of P p -> Forall_parse_of P' p
+    : Forall_parse_of P (parse_of_respectful H p) -> Forall_parse_of P' (parse_of_respectful H' p)
     with expand_forall_parse_of_production
-           str
-           (f : forall str', str' ≤s str -> forall n, P str' n -> P' str' n)
-           pat (p : parse_of_production G str pat)
+           str str' str''
+           (f : forall str0' str1', str0' ≤s str -> str0' =s str1' -> forall n, P str0' n -> P' str1' n)
+           pat (H : str =s str') (H' : str =s str'') (p : parse_of_production G str pat)
            {struct p}
-         : Forall_parse_of_production P p -> Forall_parse_of_production P' p.
+         : Forall_parse_of_production P (parse_of_production_respectful H p) -> Forall_parse_of_production P' (parse_of_production_respectful H' p).
     Proof.
-      { exact (match p in parse_of _ _ pats'
-                     return (forall str'', str'' ≤s str -> forall n, P str'' n -> P' str'' n)
-                            -> Forall_parse_of P p -> Forall_parse_of P' p
-               with
-                 | ParseHead _ _ p'
-                   => fun f' => @expand_forall_parse_of_production _ f' _ p'
-                 | ParseTail _ _ p'
-                   => fun f' => @expand_forall_parse_of _ f' _ p'
-               end f). }
-      { refine (match p in parse_of_production _ _ pats'
-                      return (forall str'', str'' ≤s str -> forall n, P str'' n -> P' str'' n)
-                             -> Forall_parse_of_production P p -> Forall_parse_of_production P' p
-                with
-                  | ParseProductionNil pf => fun _ x => x
-                  | ParseProductionCons pat strs' pats p' p''
-                    => fun f' ab
-                       => (_ : Forall_parse_of_item' _ (@Forall_parse_of _) _,
-                           expand_forall_parse_of_production
-                             _
-                             (fun str'' pf'' => f' str'' (transitivity pf'' str_le_drop))
-                             _ _
-                             (snd ab))
-                end f).
-        destruct p'; simpl.
-        { exact tt. }
-        { refine (f' _ str_le_take _ (fst (fst ab)),
-                  expand_forall_parse_of _ _ _ _ (snd (fst ab))).
-          intros ??; apply f'.
-          etransitivity; [ eassumption | exact str_le_take ]. } }
+      { destruct p.
+        simpl.
+        { apply expand_forall_parse_of_production; exact f. }
+        { refine (expand_forall_parse_of _ _ _ _ _ _ _ p); exact f. } }
+      { destruct p as [ | n pat pats pit pits ]; simpl.
+        { exact (fun x => x). }
+        { pose proof (fun f' f'' => @expand_forall_parse_of_item' _ (take n str') (take n str'') (@Forall_parse_of) (@expand_forall_parse_of _ _ _ f') f'' _ pit) as expand_forall_parse_of_item.
+          specialize (fun f' H H' => expand_forall_parse_of_production _ (drop n str') (drop n str'') f' _ H H' pits).
+          clear expand_forall_parse_of.
+          change (Forall_parse_of_item P (parse_of_item_respectful (take_Proper eq_refl H) pit) * Forall_parse_of_production P (parse_of_production_respectful (drop_Proper eq_refl H) pits)
+                  -> Forall_parse_of_item P' (parse_of_item_respectful (take_Proper eq_refl H') pit) * Forall_parse_of_production P' (parse_of_production_respectful (drop_Proper eq_refl H') pits))%type.
+          intro xy.
+          split.
+          { eapply expand_forall_parse_of_item; [ .. | exact (fst xy) ].
+            { intros ? ? H''; apply f.
+              rewrite str_le_take in H''; assumption. }
+            { intro; apply f.
+              { clear -H HSLP.
+                rewrite str_le_take, H; reflexivity. }
+              { rewrite <- H, <- H'; reflexivity. } } }
+          { eapply expand_forall_parse_of_production; [ .. | exact (snd xy) ].
+            intros ? ? H''; apply f.
+            etransitivity; [ eassumption | apply str_le_drop ]. } } }
     Defined.
 
     Global Arguments expand_forall_parse_of : simpl never.
     Global Arguments expand_forall_parse_of_production : simpl never.
 
-    Definition expand_forall_parse_of_item {str} f {it} {p : parse_of_item G str it}
-      := @expand_forall_parse_of_item' str _ (@expand_forall_parse_of str f) (f _ (reflexivity _)) it p.
+    Definition expand_forall_parse_of_item {str str' str''} f {it} {p : parse_of_item G str it} (H : str =s str') (H' : str =s str'')
+      := @expand_forall_parse_of_item' str str' str'' _ (@expand_forall_parse_of str str' str'' f) (f _ _ ((_ : Proper (beq ==> beq ==> impl) str_le) _ _ H _ _ (reflexivity _) (reflexivity _)) (transitivity (symmetry H) H')) it p.
 
     Global Arguments expand_forall_parse_of_item : simpl never.
+
+    (*Section specialized.
+      Context {str str' str''}
+              (f : forall str0' str1', str0' ≤s str -> str0' =s str1' -> forall n, P str0' n -> P' str1' n)
+
+             pats (H : str =s str') (H' : str =s str'') (p : parse_of G str pats)
+             {struct p}
+    : Forall_parse_of P (parse_of_respectful H p) -> Forall_parse_of P' (parse_of_respectful H' p)*)
   End expand.
 End cfg.
