src/Parsers/Splitters/BruteForce.v
@@ -3,19 +3,31 @@ Require Import Coq.Lists.List Coq.Strings.String.
 Require Import ADTSynthesis.Parsers.ContextFreeGrammar.
 Require Import ADTSynthesis.Parsers.BaseTypes ADTSynthesis.Parsers.BooleanBaseTypes.
 Require Import ADTSynthesis.Parsers.Splitters.RDPList.
+Require Import ADTSynthesis.Parsers.MinimalParseOfParse.
 Require Import ADTSynthesis.Common.
 
 Set Implicit Arguments.
 Local Open Scope string_like_scope.
 
 Section brute_force_splitter.
-  Context {string} {HSL : StringLike string}.
+  Context {string} {HSL : StringLike string} {HSLP : StringLikeProperties string}.
 
   Fixpoint up_to (n : nat) : list nat :=
     match n with
       | 0 => nil
       | S n' => n'::up_to n'
     end.
+
+  Lemma in_up_to {n m} (H : n < m) : List.In n (up_to m).
+  Proof.
+    revert n H; induction m; intros n H.
+    { exfalso; omega. }
+    { simpl.
+      hnf in H.
+      apply le_S_n in H.
+      apply Compare_dec.le_lt_eq_dec in H.
+      destruct H; subst; [ right; eauto | left; reflexivity ]. }
+  Qed.
 
   Definition make_all_single_splits (str : String) : list nat
     := (length str)::up_to (length str).
@@ -36,10 +48,15 @@ Section brute_force_splitter.
     destruct (Compare_dec.le_lt_dec (length str) n).
     { exists (length str); simpl; repeat split.
       { left; reflexivity. }
-      {
-      unfold make_all_single_splits.
-    SearchAbout sumbool lt.
-    destruct (lt_dec n
-    apply (@make_all_single_splits_complete G str0 valid _ _ str pf).
-  Defined.
+      { eapply expand_minimal_parse_of_item; [ .. | eassumption ];
+        try solve [ reflexivity
+                  | left; reflexivity
+                  | rewrite !take_long; trivial; reflexivity ]. }
+      { eapply expand_minimal_parse_of_production; [ .. | eassumption ];
+        try solve [ reflexivity
+                  | left; reflexivity
+                  | apply bool_eq_empty; rewrite drop_length; omega ]. } }
+    { exists n; simpl; repeat split; try assumption.
+      right; apply in_up_to; assumption. }
+  Qed.
 End brute_force_splitter.
