src/Parsers/WellFoundedParseProperties.v
@@ -1,0 +1,60 @@
+(** * Properties about well-founded relation on [parse_of] *)
+Require Import Coq.Strings.String Coq.Lists.List Coq.Program.Program Coq.Program.Wf Coq.Arith.Wf_nat Coq.Relations.Relation_Definitions.
+Require Import Coq.Classes.Morphisms.
+Require Import ADTSynthesis.Parsers.ContextFreeGrammar.
+Require Import ADTSynthesis.Parsers.ContextFreeGrammarProperties.
+Require Import ADTSynthesis.Parsers.WellFoundedParse.
+
+Set Implicit Arguments.
+
+Local Notation "R ==> R'" := (@respectful_hetero _ _ _ _ R R')
+                               (at level 55, right associativity)
+                             : dep_signature_scope.
+Delimit Scope dep_signature_scope with signatureD.
+
+Section rel.
+  Context {string} {HSL : StringLike string} {HSLP : StringLikeProperties string} {G : grammar string}.
+
+  Fixpoint size_of_parse_respectful {str str' pats} (H : str =s str') (p : parse_of G str pats)
+  : size_of_parse p = size_of_parse (parse_of_respectful H p)
+    := match p return size_of_parse p = size_of_parse (parse_of_respectful H p) with
+         | ParseHead _ _ p' => f_equal S (size_of_parse_production_respectful H p')
+         | ParseTail _ _ p' => f_equal S (size_of_parse_respectful H p')
+       end
+  with size_of_parse_production_respectful {str str' pat} (H : str =s str') (p : parse_of_production G str pat)
+       : size_of_parse_production p = size_of_parse_production (parse_of_production_respectful H p)
+       := match p return size_of_parse_production p = size_of_parse_production (parse_of_production_respectful H p) with
+            | ParseProductionNil _ => eq_refl
+            | ParseProductionCons _ _ _ _ _ => f_equal2 (fun x y => S (x + y))
+                                                        (size_of_parse_item_respectful _ _)
+                                                        (size_of_parse_production_respectful _ _)
+          end
+  with size_of_parse_item_respectful {str str' it} (H : str =s str') (p : parse_of_item G str it)
+       : size_of_parse_item p = size_of_parse_item (parse_of_item_respectful H p)
+       := match p with
+            | ParseTerminal _ _ => eq_refl
+            | ParseNonTerminal _ p' => f_equal S (size_of_parse_respectful H p')
+          end.
+
+  Global Instance size_of_parse_ProperD {pats}
+  : Proper (beq ==> (fun str str' => (fun p p' => forall H, p = parse_of_respectful H p') ==> (fun _ _ => @eq nat)))%signatureD
+           (fun str => @size_of_parse string _ G str pats).
+  Proof.
+    intros ?? H p p' H'.
+    rewrite (H' (symmetry H)).
+    rewrite <- size_of_parse_respectful; reflexivity.
+  Qed.
+
+  Global Instance size_of_parse_Proper {pats} {P : _ -> Prop}
+  : Proper (beq ==> impl)
+           (fun str =>
+              forall p : parse_of G str pats,
+                P (size_of_parse p)).
+  Proof.
+    repeat intro.
+    erewrite size_of_parse_respectful.
+    apply H0.
+    Grab Existential Variables.
+    symmetry; assumption.
+  Qed.
+End rel.
